VCVio/CryptoFoundations/AsymmEncAlg.lean
@@ -17,24 +17,31 @@ public/secret keys `PK` and `SK`, and ciphertext space `C`.
 
 open OracleSpec OracleComp
 
-structure AsymmEncAlg {ι : Type} (spec : OracleSpec ι) (M PK SK C : Type)
+structure AsymmEncAlg {ι : Type} (spec : ℕ → OracleSpec ι)
+    (M PK SK C : ℕ → Type)
     extends OracleAlg spec where
-  keygen : Unit → OracleComp spec (PK × SK)
-  encrypt : M → PK → OracleComp spec C
-  decrypt : C → SK → OracleComp spec M
+  keygen (sp : ℕ) : OracleComp (spec sp) (PK sp × SK sp)
+  encrypt (sp : ℕ) : M sp → PK sp → OracleComp (spec sp) (C sp)
+  decrypt (sp : ℕ) : C sp → SK sp → OracleComp (spec sp) (M sp)
 
 namespace AsymmEncAlg
 
-variable {ι : Type} {spec : OracleSpec ι} {M PK SK C : Type}
+variable {ι : Type} {spec : ℕ → OracleSpec ι} {M PK SK C : ℕ → Type}
+
+section sound
+
+variable [Π sp, DecidableEq (M sp)]
 
 /-- Experiment for checking that an asymmetric encryption algorithm is sound,
 i.e. that decryption properly reverses encryption -/
-def soundnessExp [DecidableEq M] (encAlg : AsymmEncAlg spec M PK SK C)
-    (m : M) : SecExp spec (PK × SK) where
-  inpGen := encAlg.keygen ()
-  main := λ (pk, sk) ↦ do
-    let σ ← encAlg.encrypt m pk
-    let m' ← encAlg.decrypt σ sk
+def soundnessExp (encAlg : AsymmEncAlg spec M PK SK C)
+    (mDist : (sp : ℕ) → OracleComp (spec sp) (M sp)) :
+    SecExp spec where
+  main := λ sp ↦ do
+    let m ← mDist sp
+    let (pk, sk) ← encAlg.keygen sp
+    let σ ← encAlg.encrypt sp m pk
+    let m' ← encAlg.decrypt sp σ sk
     return m = m'
   __ := encAlg
 
@@ -44,16 +51,18 @@ namespace soundnessExp
 end soundnessExp
 
 /-- An asymmetric encryption algorithm is sound if messages always decrypt to themselves. -/
-def isSound [DecidableEq M] (encAlg : AsymmEncAlg spec M PK SK C) : Prop :=
-  ∀ m : M, (soundnessExp encAlg m).advantage = 1
+def isSound (encAlg : AsymmEncAlg spec M PK SK C) : Prop :=
+  ∀ mDist, negligible (1 - (soundnessExp encAlg mDist).advantage)
 
-lemma sound_iff [DecidableEq M] (encAlg : AsymmEncAlg spec M PK SK C) : encAlg.isSound ↔
-    ∀ m : M, ∀ m' ∈ (encAlg.exec <| do
-      let (pk, sk) ← encAlg.keygen ()
-      let σ ← encAlg.encrypt m pk
-      encAlg.decrypt σ sk).support, m = m' := by
-  simp only [isSound, SecExp.advantage_eq_one_iff]
-  sorry
+-- lemma sound_iff [DecidableEq M] (encAlg : AsymmEncAlg spec M PK SK C) : encAlg.isSound ↔
+--     ∀ m : M, ∀ m' ∈ (encAlg.exec <| do
+--       let (pk, sk) ← encAlg.keygen ()
+--       let σ ← encAlg.encrypt m pk
+--       encAlg.decrypt σ sk).support, m = m' := by
+--   simp only [isSound, SecExp.advantage_eq_one_iff]
+--   sorry
+
+end sound
 
 section IND_CPA
 
@@ -64,9 +73,9 @@ it can distinguish the encryption of. It addionally has a `distinguish` function
 that given a pair of messages and an encryption, returns whether it is an encryption of
 the first message or the second message. -/
 structure IND_CPA_Adv (encAlg : AsymmEncAlg spec M PK SK C)
-    extends SecAdv spec PK (M × M) where
-  distinguish : PK → M × M → C → OracleComp spec Bool
-  -- (distinguish_qb : query_count spec)
+    extends SecAdv spec (λ sp ↦ PK sp) (λ sp ↦ M sp × M sp) where
+  distinguish (sp : ℕ) : PK sp → M sp × M sp →
+    C sp → OracleComp (spec sp) Bool
 
 /-- Experiment for IND-CPA security of an asymmetric encryption algorithm.
 `inp_gen` generates a key and pre-selects a random boolean value.
@@ -74,17 +83,16 @@ structure IND_CPA_Adv (encAlg : AsymmEncAlg spec M PK SK C)
 the boolean chosen in `inp_gen`, finally asking the adversary to determine the boolean
 given the messages and resulting ciphertext. `is_valid` checks that this choice is correct.
 The simulation oracles are pulled in directly from the encryption algorithm. -/
-def IND_CPA_Exp [coinSpec ⊂ₒ spec] {encAlg : AsymmEncAlg spec M PK SK C}
-    (adv : IND_CPA_Adv encAlg) : SecExp spec (PK × Bool) where
-  inpGen := do
-    let ⟨pk, _⟩ ← encAlg.keygen ()
-    -- let b ← ↑coin TODO: fix
-    return (pk, true)
-  main := λ ⟨pk, b⟩ ↦ do
-    let ⟨m₁, m₂⟩ ← adv.run pk
+def IND_CPA_Exp {encAlg : AsymmEncAlg spec M PK SK C}
+    (adv : IND_CPA_Adv encAlg) :
+    SecExp spec where
+  main := λ sp ↦ do
+    let ⟨pk, _⟩ ← encAlg.keygen sp
+    let ⟨m₁, m₂⟩ ← adv.run sp pk
+    let b : Bool := true -- fix
     let m := if b then m₁ else m₂
-    let c ← encAlg.encrypt m pk
-    let b' ← adv.distinguish pk (m₁, m₂) c
+    let c ← encAlg.encrypt sp m pk
+    let b' ← adv.distinguish sp pk (m₁, m₂) c
     return b = b'
   __ := encAlg
 
