VCVio/CryptoFoundations/HardnessAssumptions/HardHomogeneousSpace.lean
@@ -5,7 +5,6 @@ Authors: Devon Tuma
 -/
 import VCVio.CryptoFoundations.SecExp
 import VCVio.CryptoFoundations.Negligible
--- import VCVio.OracleComp.Constructions.UniformSelect
 
 /-!
 # Hard Homogeneous Spaces
@@ -18,10 +17,7 @@ and extend this with finiteness and decidability conditions
 
 open OracleSpec OracleComp OracleAlg BigOperators ENNReal
 
-section testing
-
-
-class HomogeneousSpace' (G : semiOutParam (ℕ → Type))
+class HomogeneousSpace (G : semiOutParam (ℕ → Type))
     (P : semiOutParam (ℕ → Type)) :=
   AddGroup_G (sp : ℕ) : AddGroup (G sp)
   AddTorsor_GP (sp : ℕ) : AddTorsor (G sp) (P sp)
@@ -34,126 +30,99 @@ class HomogeneousSpace' (G : semiOutParam (ℕ → Type))
   selectableType_G (sp : ℕ) : SelectableType (G sp)
   selectableType_P (sp : ℕ) : SelectableType (P sp)
 
+namespace HomogeneousSpace
+
 variable (G P : ℕ → Type)
 
-instance [h : HomogeneousSpace' G P] (sp : ℕ) : AddGroup (G sp) := h.AddGroup_G sp
-instance [h : HomogeneousSpace' G P] (sp : ℕ) : AddTorsor (G sp) (P sp) := h.AddTorsor_GP sp
-instance [h : HomogeneousSpace' G P] (sp : ℕ) : DecidableEq (G sp) := h.decidableEq_G sp
-instance [h : HomogeneousSpace' G P] (sp : ℕ) : DecidableEq (P sp) := h.decidableEq_P sp
-instance [h : HomogeneousSpace' G P] (sp : ℕ) : Fintype (G sp) := h.fintype_G sp
-instance [h : HomogeneousSpace' G P] (sp : ℕ) : Fintype (P sp) := h.fintype_P sp
-instance [h : HomogeneousSpace' G P] (sp : ℕ) : Inhabited (G sp) := h.inhabited_G sp
-instance [h : HomogeneousSpace' G P] (sp : ℕ) : Inhabited (P sp) := h.inhabited_P sp
-instance [h : HomogeneousSpace' G P] (sp : ℕ) : SelectableType (G sp) := h.selectableType_G sp
-instance [h : HomogeneousSpace' G P] (sp : ℕ) : SelectableType (P sp) := h.selectableType_P sp
+instance [h : HomogeneousSpace G P] (sp : ℕ) : AddGroup (G sp) := h.AddGroup_G sp
+instance [h : HomogeneousSpace G P] (sp : ℕ) : AddTorsor (G sp) (P sp) := h.AddTorsor_GP sp
+instance [h : HomogeneousSpace G P] (sp : ℕ) : DecidableEq (G sp) := h.decidableEq_G sp
+instance [h : HomogeneousSpace G P] (sp : ℕ) : DecidableEq (P sp) := h.decidableEq_P sp
+instance [h : HomogeneousSpace G P] (sp : ℕ) : Fintype (G sp) := h.fintype_G sp
+instance [h : HomogeneousSpace G P] (sp : ℕ) : Fintype (P sp) := h.fintype_P sp
+instance [h : HomogeneousSpace G P] (sp : ℕ) : Inhabited (G sp) := h.inhabited_G sp
+instance [h : HomogeneousSpace G P] (sp : ℕ) : Inhabited (P sp) := h.inhabited_P sp
+instance [h : HomogeneousSpace G P] (sp : ℕ) : SelectableType (G sp) := h.selectableType_G sp
+instance [h : HomogeneousSpace G P] (sp : ℕ) : SelectableType (P sp) := h.selectableType_P sp
 
-structure SecAdv' {ι : Type}
-    (spec : ℕ → OracleSpec ι)
-    (α β : ℕ → Type) where
-  run (sp : ℕ) : α sp → OracleComp (spec sp) (β sp)
+section vectorization
 
-structure OracleAlg' {ι : Type} (spec : ℕ → OracleSpec ι) where
-  baseState (sp : ℕ) : Type
-  init_state (sp : ℕ) : baseState sp
-  baseSimOracle (sp : ℕ) : spec sp →[baseState sp]ₛₒ unifSpec
+def vectorizationAdv (G P : (sp : ℕ) → Type) :=
+  SecAdv (λ _ ↦ unifSpec) (λ sp ↦ P sp × P sp) (λ sp ↦ G sp)
 
-@[inline, reducible]
-def baseOracleAlg' : OracleAlg' (λ _ ↦ unifSpec) where
-  baseState := λ _ ↦ Unit
-  init_state := λ _ ↦ ()
-  baseSimOracle := λ _ ↦ idOracle
-
-structure SecExp' {ι : Type} (spec : ℕ → OracleSpec ι)
-    -- (α : ℕ → Type)
-    extends OracleAlg' spec where
-  -- inpGen (sp : ℕ) : OracleComp (spec sp) (α sp)
-  main (sp : ℕ) : OracleComp (spec sp) Bool
-
-def SecExp'.runExp {ι : Type} {spec : ℕ → OracleSpec ι}
-    (exp : SecExp' spec) (sp : ℕ) : OracleComp unifSpec Bool :=
-  simulate' (exp.baseSimOracle sp)
-    (exp.init_state sp) (exp.main sp)
-
-def VectorizationAdv' (G P : (sp : ℕ) → Type) :=
-  SecAdv' (λ _ ↦ unifSpec) (λ sp ↦ P sp × P sp) (λ sp ↦ G sp)
-
-def vectorizationExp' (G P : ℕ → Type)
-    [HomogeneousSpace' G P]
-    (adv : VectorizationAdv' G P) :
-    SecExp' (λ _ ↦ unifSpec) where
+def vectorizationExp (G P : ℕ → Type)
+    [HomogeneousSpace G P]
+    (adv : vectorizationAdv G P) :
+    SecExp (λ _ ↦ unifSpec) where
   main := λ sp ↦ do
     let x₁ ← $ᵗ P sp
     let x₂ ← $ᵗ P sp
     let g ← adv.run sp (x₁, x₂)
     return g = x₁ -ᵥ x₂
-  __ := baseOracleAlg'
-
-noncomputable def vectorizationAdvantage' (G P : ℕ → Type)
-    [HomogeneousSpace' G P]
-    (adv : VectorizationAdv' G P) (sp : ℕ) : ℝ≥0∞ :=
-    [= true | (vectorizationExp' G P adv).runExp sp]
-
-def vectorizationHard' (G P : ℕ → Type)
-    [HomogeneousSpace' G P] : Prop :=
-  ∀ adv, negligible (λ sp ↦ vectorizationAdvantage' G P adv sp)
-
-end testing
-
-/-- A `HomogeneousSpace G P` is a group action of a group `G` on a set of points `P`,
-such that the action induces a bijection (represented by the `AddTorsor` class),
-with the additional assumption that both spaces are finite. -/
-class HomogeneousSpace (G : outParam Type) (P : semiOutParam Type)
-    [outParam (AddGroup G)]
-    extends AddTorsor G P where
-  decidableEq_G : DecidableEq G
-  decidableEq_P : DecidableEq P
-  fintype_G : Fintype G
-  fintype_P : Fintype P
-  inhabited_G : Inhabited G
-  inhabited_P : Inhabited P
-  selectableType_G : SelectableType G
-  selectableType_P : SelectableType P
-
-namespace HomogeneousSpace
-
-variable {G P : Type} [AddGroup G]
-
-instance [h : HomogeneousSpace G P] : DecidableEq G := h.decidableEq_G
-instance [h : HomogeneousSpace G P] : DecidableEq P := h.decidableEq_P
-instance [h : HomogeneousSpace G P] : Fintype G := h.fintype_G
-instance [h : HomogeneousSpace G P] : Fintype P := h.fintype_P
-instance [h : HomogeneousSpace G P] : Inhabited G := h.inhabited_G
-instance [h : HomogeneousSpace G P] : Inhabited P := h.inhabited_P
-instance [h : HomogeneousSpace G P] : SelectableType G := h.selectableType_G
-instance [h : HomogeneousSpace G P] : SelectableType P := h.selectableType_P
-
-/-- An adversary for the vectorization game takes in a pair of base points `(x₁, x₂)`,
-and attempts to generate a vectorization, i.g. a vector `g` with `g +ᵥ x₂ = x₁`.
-
-TODO: how does ":=" compare to "extends" in practice? -/
-structure vectorizationAdv (G P : Type)
-  extends SecAdv unifSpec (P × P) G
-
-/-- Analogue of the game for the discrete logarithm assumption.
-The input generator randomly chooses the challenge points for the adversary,
-and a result is valid if it is exactly the vectorization of the challenge points. -/
-noncomputable def vectorizationExp [HomogeneousSpace G P]
-    (adv : vectorizationAdv G P) : SecExp unifSpec (P × P) where
-  inpGen := (·, ·) <$> ($ᵗ P) <*> ($ᵗ P)
-  main := λ (x₁, x₂) ↦ do
-    let g ← adv.run (x₁, x₂)
-    return g = x₁ -ᵥ x₂
   __ := baseOracleAlg
 
-namespace vectorizationExp
+def vectorizationHard (G P : ℕ → Type) [HomogeneousSpace G P] : Prop :=
+  ∀ adv : vectorizationAdv G P, negligible (vectorizationExp G P adv).advantage
 
-@[simp]
-lemma advantage_eq [HomogeneousSpace G P] (adv : vectorizationAdv G P) :
-    (vectorizationExp adv).advantage =
-      ∑ x₁ : P, ∑ x₂ : P, [= x₁ -ᵥ x₂ | adv.run (x₁, x₂)] / (Fintype.card P) ^ 2 := by
-  simp [vectorizationExp, Finset.mul_sum]
-  sorry
-
-end vectorizationExp
+end vectorization
 
 end HomogeneousSpace
+
+-- /-- A `HomogeneousSpace G P` is a group action of a group `G` on a set of points `P`,
+-- such that the action induces a bijection (represented by the `AddTorsor` class),
+-- with the additional assumption that both spaces are finite. -/
+-- class HomogeneousSpace (G : outParam Type) (P : semiOutParam Type)
+--     [outParam (AddGroup G)]
+--     extends AddTorsor G P where
+--   decidableEq_G : DecidableEq G
+--   decidableEq_P : DecidableEq P
+--   fintype_G : Fintype G
+--   fintype_P : Fintype P
+--   inhabited_G : Inhabited G
+--   inhabited_P : Inhabited P
+--   selectableType_G : SelectableType G
+--   selectableType_P : SelectableType P
+
+-- namespace HomogeneousSpace
+
+-- variable {G P : Type} [AddGroup G]
+
+-- instance [h : HomogeneousSpace G P] : DecidableEq G := h.decidableEq_G
+-- instance [h : HomogeneousSpace G P] : DecidableEq P := h.decidableEq_P
+-- instance [h : HomogeneousSpace G P] : Fintype G := h.fintype_G
+-- instance [h : HomogeneousSpace G P] : Fintype P := h.fintype_P
+-- instance [h : HomogeneousSpace G P] : Inhabited G := h.inhabited_G
+-- instance [h : HomogeneousSpace G P] : Inhabited P := h.inhabited_P
+-- instance [h : HomogeneousSpace G P] : SelectableType G := h.selectableType_G
+-- instance [h : HomogeneousSpace G P] : SelectableType P := h.selectableType_P
+
+-- /-- An adversary for the vectorization game takes in a pair of base points `(x₁, x₂)`,
+-- and attempts to generate a vectorization, i.g. a vector `g` with `g +ᵥ x₂ = x₁`.
+
+-- TODO: how does ":=" compare to "extends" in practice? -/
+-- structure vectorizationAdv (G P : Type)
+--   extends SecAdv unifSpec (P × P) G
+
+-- /-- Analogue of the game for the discrete logarithm assumption.
+-- The input generator randomly chooses the challenge points for the adversary,
+-- and a result is valid if it is exactly the vectorization of the challenge points. -/
+-- noncomputable def vectorizationExp [HomogeneousSpace G P]
+--     (adv : vectorizationAdv G P) : SecExp unifSpec (P × P) where
+--   inpGen := (·, ·) <$> ($ᵗ P) <*> ($ᵗ P)
+--   main := λ (x₁, x₂) ↦ do
+--     let g ← adv.run (x₁, x₂)
+--     return g = x₁ -ᵥ x₂
+--   __ := baseOracleAlg
+
+-- namespace vectorizationExp
+
+-- @[simp]
+-- lemma advantage_eq [HomogeneousSpace G P] (adv : vectorizationAdv G P) :
+--     (vectorizationExp adv).advantage =
+--       ∑ x₁ : P, ∑ x₂ : P, [= x₁ -ᵥ x₂ | adv.run (x₁, x₂)] / (Fintype.card P) ^ 2 := by
+--   simp [vectorizationExp, Finset.mul_sum]
+--   sorry
+
+-- end vectorizationExp
+
+-- end HomogeneousSpace
