VCVio/CryptoFoundations/SecExp.lean
@@ -5,6 +5,7 @@ Authors: Devon Tuma
 -/
 import VCVio.OracleComp.OracleAlg
 import VCVio.OracleComp.Constructions.UniformSelect
+import VCVio.CryptoFoundations.Negligible
 
 /-!
 # Security Experiments
@@ -26,14 +27,19 @@ open OracleComp OracleSpec ENNReal
 
 /-- A security adversary bundling a computation with a bound on the number of queries it makes.
 This is useful both for asymptotic security as well as in some concrete security bounds. -/
-structure SecAdv {ι : Type} (spec : OracleSpec ι)
-    (α β : Type) where
-  run : α → OracleComp spec β
-  -- run_polyTime : polyTimeOracleComp run
-  queryBound : ι → ℕ
-  -- queryBound_isQueryBound (x : α) : IsQueryBound (run x) queryBound
-  activeOracles : List ι -- Canonical ordering of oracles
-  -- mem_activeOracles_iff : ∀ i, i ∈ activeOracles ↔ queryBound i ≠ 0
+-- structure SecAdv {ι : Type} (spec : OracleSpec ι)
+--     (α β : Type) where
+--   run : α → OracleComp spec β
+--   -- run_polyTime : polyTimeOracleComp run
+--   queryBound : ι → ℕ
+--   -- queryBound_isQueryBound (x : α) : IsQueryBound (run x) queryBound
+--   activeOracles : List ι -- Canonical ordering of oracles
+--   -- mem_activeOracles_iff : ∀ i, i ∈ activeOracles ↔ queryBound i ≠ 0
+
+structure SecAdv {ι : Type}
+    (spec : ℕ → OracleSpec ι)
+    (α β : ℕ → Type) where
+  run (sp : ℕ) : α sp → OracleComp (spec sp) (β sp)
 
 namespace SecAdv
 
@@ -41,37 +47,45 @@ variable {ι : Type} {spec : OracleSpec ι} {α β : Type}
 
 end SecAdv
 
-/-- A security experiment using oracles in `spec`, represented as an `OracleAlg`. -/
-structure SecExp {ι : Type} (spec : OracleSpec ι) (α : Type)
+
+structure SecExp {ι : Type} (spec : ℕ → OracleSpec ι)
+    -- (α : ℕ → Type)
     extends OracleAlg spec where
-  inpGen : OracleComp spec α
-  main : α → OracleComp spec Bool
+  -- inpGen (sp : ℕ) : OracleComp (spec sp) (α sp)
+  main (sp : ℕ) : OracleComp (spec sp) Bool
+
+
+-- /-- A security experiment using oracles in `spec`, represented as an `OracleAlg`. -/
+-- structure SecExp {ι : Type} (spec : ℕ → OracleSpec ι) (α : Type)
+--     extends OracleAlg spec where
+--   inpGen : OracleComp spec α
+--   main : α → OracleComp spec Bool
 
 namespace SecExp
 
-variable {ι : Type} {spec : OracleSpec ι} {α β : Type}
+variable {ι : Type} {spec : ℕ → OracleSpec ι} {α β : Type}
 
-noncomputable def advantage (exp : SecExp spec α) : ℝ≥0∞ :=
-    [= true | exp.exec (exp.inpGen >>= exp.main)]
+noncomputable def advantage (exp : SecExp spec) (sp : ℕ) : ℝ≥0∞ :=
+    [= true | exp.exec sp (exp.main sp)]
 
-lemma advantage_eq (exp : SecExp spec α) :
-    exp.advantage = [= true | exp.exec (exp.inpGen >>= exp.main)] := rfl
+-- lemma advantage_eq (exp : SecExp spec α) :
+--     exp.advantage = [= true | exp.exec (exp.inpGen >>= exp.main)] := rfl
 
-@[simp]
-lemma advantage_eq_one_iff (exp : SecExp spec α) : exp.advantage = 1 ↔
-    false ∉ (exp.exec (exp.inpGen >>= exp.main)).support := by
-  simp only [advantage_eq, probOutput_eq_one_iff, OracleAlg.exec_bind, support_bind,
-    Set.subset_singleton_iff, Set.mem_iUnion, exists_prop, Prod.exists, forall_exists_index,
-    and_imp, Bool.forall_bool, imp_false, implies_true, and_true, not_exists, not_and]
+-- @[simp]
+-- lemma advantage_eq_one_iff (exp : SecExp spec α) : exp.advantage = 1 ↔
+--     false ∉ (exp.exec (exp.inpGen >>= exp.main)).support := by
+--   simp only [advantage_eq, probOutput_eq_one_iff, OracleAlg.exec_bind, support_bind,
+--     Set.subset_singleton_iff, Set.mem_iUnion, exists_prop, Prod.exists, forall_exists_index,
+--     and_imp, Bool.forall_bool, imp_false, implies_true, and_true, not_exists, not_and]
 
-@[simp]
-lemma advantage_eq_zero_iff (exp : SecExp spec α) : exp.advantage = 0 ↔
-    true ∉ (exp.exec (exp.inpGen >>= exp.main)).support := by
-  rw [advantage_eq, probOutput_eq_zero_iff]
+-- @[simp]
+-- lemma advantage_eq_zero_iff (exp : SecExp spec α) : exp.advantage = 0 ↔
+--     true ∉ (exp.exec (exp.inpGen >>= exp.main)).support := by
+--   rw [advantage_eq, probOutput_eq_zero_iff]
 
-@[simp]
-lemma advantage_pos_iff (exp : SecExp spec α) : 0 < exp.advantage ↔
-    true ∈ (exp.exec (exp.inpGen >>= exp.main)).support := by
-  rw [pos_iff_ne_zero, ne_eq, advantage_eq_zero_iff, not_not]
+-- @[simp]
+-- lemma advantage_pos_iff (exp : SecExp spec α) : 0 < exp.advantage ↔
+--     true ∈ (exp.exec (exp.inpGen >>= exp.main)).support := by
+--   rw [pos_iff_ne_zero, ne_eq, advantage_eq_zero_iff, not_not]
 
 end SecExp
